{
 "cells": [
  {
   "cell_type": "code",
   "execution_count": 1,
   "metadata": {},
   "outputs": [],
   "source": [
    "%load_ext autoreload\n",
    "%autoreload 2\n",
    "%reload_ext autoreload\n",
    "%matplotlib inline"
   ]
  },
  {
   "cell_type": "markdown",
   "metadata": {},
   "source": [
    "# Author: Giorgi Sharmiashvili"
   ]
  },
  {
   "cell_type": "markdown",
   "metadata": {},
   "source": [
    "# Sigma-algebras"
   ]
  },
  {
   "cell_type": "markdown",
   "metadata": {},
   "source": [
    "#### Prove that:\n",
    "Composition of mesurable functions is a mesurable function"
   ]
  },
  {
   "cell_type": "markdown",
   "metadata": {},
   "source": [
    "- Let ${f:X \\to Y, g: Y \\to Z}$ be a measurable functions. Let S be subset from Z. If ${S \\in Z}$ then ${g^{-1}(S) \\in Y \\to (g \\circ f)^{-1}(S) = f^{-1}(g^{-1}(S) \\in X}$"
   ]
  },
  {
   "cell_type": "markdown",
   "metadata": {},
   "source": [
    "--------------------------------"
   ]
  },
  {
   "cell_type": "markdown",
   "metadata": {},
   "source": [
    "## Mesure"
   ]
  },
  {
   "cell_type": "markdown",
   "metadata": {},
   "source": [
    "#### Prove the following mesure properties:\n",
    "- if $A \\subset B$ then $\\mu(A) \\le \\mu(B)$\n"
   ]
  },
  {
   "cell_type": "markdown",
   "metadata": {},
   "source": [
    "- $(B - A) \\cup (A \\cap B) = (B - A) \\cup A = B$ and $(B - A) \\cap (A \\cap B) = \\emptyset$ so $\\mu((B - A) \\cup (A \\cap B)) = \\mu(B - A) + \\mu(A \\cap B) = \\mu(B - A) + \\mu(A) = \\mu(B)$ so $\\mu(A) \\le \\mu(B)$"
   ]
  },
  {
   "cell_type": "markdown",
   "metadata": {},
   "source": [
    "------------------------------"
   ]
  },
  {
   "cell_type": "markdown",
   "metadata": {},
   "source": [
    "## Probability"
   ]
  },
  {
   "cell_type": "markdown",
   "metadata": {},
   "source": [
    "#### Prove that:\n",
    "For probability mesure $P$ and events $A, B, C \\subset \\Omega$\n",
    "- $P(A \\cup B) = P(A) + P(B) - P(A \\cap B)$\n",
    "<br>"
   ]
  },
  {
   "cell_type": "markdown",
   "metadata": {},
   "source": [
    "- ${A = A \\cup \\Omega = A \\cap (B \\cup \\bar{B}) = (A \\cap B) \\cup (A \\cap \\bar{B})}$ \n",
    "    <br>${P(A) = P(A \\cap B) + P(A \\cap \\bar{B})}$\n",
    "    <br>${A \\cup B = (A \\cup B) \\cap (B \\cup \\bar{B}) = (A \\cap \\bar{B}) \\cup B = (A \\cap \\bar{B}) \\cup (B \\cap (A \\cup \\bar{A})) = (A \\cap \\bar{B}) \\cup (B \\cap \\bar{A}) \\cup (A \\cap B)}$\n",
    "    <br>${P(A \\cup B) = P(A \\cap \\bar{B}) + P(B \\cap \\bar{A}) + P(A \\cap B) = P(A) - P(A \\cap B) + P(B) - P(A \\cap B) + P(A \\cap B) = P(A) + P(B) - P(A \\cap B)}$"
   ]
  },
  {
   "cell_type": "markdown",
   "metadata": {},
   "source": [
    "---------------------------------------"
   ]
  },
  {
   "cell_type": "markdown",
   "metadata": {},
   "source": [
    "## Random variable"
   ]
  },
  {
   "cell_type": "markdown",
   "metadata": {},
   "source": [
    "#### Prove that:\n",
    "$$\n",
    "\\sigma^2 = \\operatorname{E}[X^2] - (\\operatorname{E}[X])^2\n",
    "$$\n",
    "Assuming that expectation exists\n",
    "<br>\n",
    "Denoted by $\\sigma^2$\n",
    "<br>"
   ]
  },
  {
   "cell_type": "markdown",
   "metadata": {},
   "source": [
    "- E[X] = $\\mu$\n",
    "    <br>E[aX + b] = aE[X] + b\n",
    "    <br>${\\sigma^2 = E[(X - \\mu)^2] = E[(X^2 - X\\mu + \\mu^2)]= E[X^2 - \\mu^2] = E[X^2] - \\mu^2 = E[X^2] - (E[X])^2}$"
   ]
  },
  {
   "cell_type": "markdown",
   "metadata": {},
   "source": [
    "--------------------------------------------"
   ]
  }
 ],
 "metadata": {
  "kernelspec": {
   "display_name": "Python 3",
   "language": "python",
   "name": "python3"
  },
  "language_info": {
   "codemirror_mode": {
    "name": "ipython",
    "version": 3
   },
   "file_extension": ".py",
   "mimetype": "text/x-python",
   "name": "python",
   "nbconvert_exporter": "python",
   "pygments_lexer": "ipython3",
   "version": "3.7.4"
  }
 },
 "nbformat": 4,
 "nbformat_minor": 4
}
